Started work on trying to do the refinement proofs for some of the higher order functions, also cleaned up some definitions to make some of the proofs shorter and faster

cogent/examples/wa_connect/Manual_AllRefine.thy
@@ -3,10 +3,10 @@ theory Manual_AllRefine
 begin
 
 
-thm  Generated_cogent_shallow.corres_shallow_C_wordarray_put2_u32[no_vars, simplified]
-thm  Generated_cogent_shallow.corres_shallow_C_wordarray_length_u32[no_vars, simplified]
-thm  Generated_cogent_shallow.corres_shallow_C_wordarray_get_u32[no_vars, simplified]
-
+thm  Generated_cogent_shallow.corres_shallow_C_wordarray_put2_u32[no_vars]
+thm  Generated_cogent_shallow.corres_shallow_C_wordarray_length_u32[no_vars]
+thm  Generated_cogent_shallow.corres_shallow_C_wordarray_get_u32[no_vars]
+thm Generated_cogent_shallow.corres_shallow_C_sum_arr[no_vars]
 section "Shallow Word Array Value Relation"
 
 overloading
@@ -47,64 +47,49 @@ definition upd_wordarray_put2_0
   "upd_wordarray_put2_0 x y =
       (let (x1, x2) = x;
            (y1, y2) = y
-      in
-        (case x2 of URecord [(UPtr p r, _), (UPrim (LU32 idx), _ ), (UPrim (LU32 val), _)] 
-              \<Rightarrow> (\<lambda>l. (case x1 p of option.Some (UAbstract (WAU32 len arr))
-                            \<Rightarrow> (if l = arr + 4 * idx \<and> idx < len 
-                                  then option.Some (UPrim (LU32 val)) else x1 l)
-                       | _ \<Rightarrow> x1 l)) = y1 \<and> UPtr p r = y2
-          | _ \<Rightarrow> False))" 
-
+      in (\<exists>p idx val. x2 = URecord [
+          (UPtr p (RCon ''WordArray'' [RPrim (Num U32)]), RPtr (RCon ''WordArray'' [RPrim (Num U32)])),
+          (UPrim (LU32 idx), RPrim (Num U32)), (UPrim (LU32 val), RPrim (Num U32))] \<and>
+          y2 = UPtr p (RCon ''WordArray'' [RPrim (Num U32)]) \<and>
+          y1 = (\<lambda>l. (if \<exists>len arr. x1 p = option.Some (UAbstract (WAU32 len arr)) \<and> 
+                        l = arr + 4 * idx \<and> idx < len then option.Some (UPrim (LU32 val)) else x1 l))))"
 
 definition upd_wordarray_get_0
   where
   "upd_wordarray_get_0 x y =
       (let (x1, x2) = x;
            (y1, y2) = y
-      in
-        (case x2 of URecord [(UPtr p r, _), (UPrim (LU32 idx), _ )] 
-              \<Rightarrow> (case x1 p of option.Some (UAbstract (WAU32 len arr))
-                        \<Rightarrow> (if idx < len then x1 (arr + 4 * idx) = option.Some y2 
-                            else y2 = UPrim (LU32 0))
-                    | _ \<Rightarrow> False) \<and> x1 = y1      
-          | _ \<Rightarrow> False))" 
+      in x1 = y1 \<and> (\<exists>p idx len arr. x2 = URecord [
+          (UPtr p (RCon ''WordArray'' [RPrim (Num U32)]), RPtr (RCon ''WordArray'' [RPrim (Num U32)])),
+          (UPrim (LU32 idx), RPrim (Num U32))] \<and> x1 p = option.Some (UAbstract (WAU32 len arr)) \<and> 
+            (idx < len \<longrightarrow> x1 (arr + 4 * idx) = option.Some y2) \<and>
+            (\<not> idx < len \<longrightarrow> y2 = UPrim (LU32 0))))"
 
 definition upd_wordarray_length_0
   where
   "upd_wordarray_length_0 x y =
       (let (x1, x2) = x;
            (y1, y2) = y
-      in
-        (case x2 of UPtr p r
-              \<Rightarrow> (case x1 p of option.Some (UAbstract (WAU32 len arr))
-                        \<Rightarrow> y2 = UPrim (LU32 len)
-                    | _ \<Rightarrow> False) \<and> x1 = y1      
-          | _ \<Rightarrow> False))" 
+      in x1 = y1 \<and> (\<exists>p len arr. x2 = UPtr p (RCon ''WordArray'' [RPrim (Num U32)]) \<and>
+          x1 p = option.Some (UAbstract (WAU32 len arr)) \<and> y2 = UPrim (LU32 len)))"
 
 definition val_wordarray_length_0
   where
-  "val_wordarray_length_0 x y =
-      (case x of VAbstract (VWA xs) 
-              \<Rightarrow> (case y of VPrim (LU32 len) 
-                        \<Rightarrow> length xs = unat len
-                    | _ \<Rightarrow> False)
-          | _ \<Rightarrow> False)" 
+  "val_wordarray_length_0 x y = (\<exists>xs len. x = VAbstract (VWA xs) \<and> y = VPrim (LU32 len) \<and> 
+                                length xs = unat len)" 
 
 
 definition val_wordarray_get_0
   where
   "val_wordarray_get_0 x y =
-      (case x of VRecord [VAbstract (VWA xs), VPrim (LU32 idx)] 
-              \<Rightarrow> (if unat idx < length xs then xs ! unat idx = y \<and> (\<exists>v. y = VPrim (LU32 v))
-                  else y = VPrim (LU32 0))
-          | _ \<Rightarrow> False)" 
+      (\<exists>xs idx v. x = VRecord [VAbstract (VWA xs), VPrim (LU32 idx)] \<and> y = VPrim (LU32 v) \<and>
+       (unat idx < length xs \<longrightarrow> xs ! unat idx = y) \<and> (\<not> unat idx < length xs \<longrightarrow> v = 0))" 
 
 definition val_wordarray_put2_0
   where
   "val_wordarray_put2_0 x y =
-      (case x of VRecord [VAbstract (VWA xs), VPrim (LU32 idx), VPrim (LU32 val)] 
-              \<Rightarrow>  VAbstract (VWA (xs[unat idx := VPrim (LU32 val)])) = y
-          | _ \<Rightarrow> False)" 
+      (\<exists>xs idx val. x = VRecord [VAbstract (VWA xs), VPrim (LU32 idx), VPrim (LU32 val)] \<and>
+       y = VAbstract (VWA (xs[unat idx := VPrim (LU32 val)])))" 
 
 
 definition \<xi>0 :: "(char list, atyp, 32 word) uabsfuns" 
@@ -226,6 +211,233 @@ sublocale WordArray \<subseteq> Generated_cogent_shallow _ abs_repr_u abs_typing
 
 context WordArray begin
 
+
+section "Naturally True Shared Assumptions for Isabelle to C Correspondence Lemmas"
+
+lemma value_sem_rename_mono_prog_rename_\<Xi>_\<xi>m_\<xi>p: 
+  "value_sem.rename_mono_prog abs_typing_v rename \<Xi> \<xi>m \<xi>p"
+  apply (clarsimp simp: val.rename_mono_prog_def)
+  apply (rule_tac x = v' in exI)
+  apply (subst (asm) rename_def)
+  apply (clarsimp simp: \<xi>m_def \<xi>p_def)
+  apply (subst (asm) assoc_lookup.simps)+
+  apply (clarsimp split: if_split_asm)
+    apply (clarsimp simp: val_wordarray_put2_0_def)
+    apply (case_tac v; clarsimp)
+    apply (case_tac z; clarsimp)
+    apply (case_tac za; clarsimp)
+    apply (case_tac zb; clarsimp)
+   apply (clarsimp simp: val_wordarray_get_0_def)
+   apply (case_tac v; clarsimp)
+   apply (case_tac z; clarsimp)
+   apply (case_tac za; clarsimp)
+  apply (clarsimp simp: val_wordarray_length_0_def)
+  apply (case_tac v; clarsimp)
+  done
+
+lemma val_proc_env_matches_\<xi>m_\<Xi>:
+  "val.proc_env_matches \<xi>m \<Xi>"
+  apply (clarsimp simp: val.proc_env_matches_def \<xi>m_def)
+  apply (subst (asm) \<Xi>_def)
+  apply (subst (asm) assoc_lookup.simps)+
+  apply (clarsimp split: if_split_asm)
+    apply (clarsimp simp: wordarray_get_0_type_def abbreviatedType6_def \<xi>m_def val_wordarray_get_0_def)
+    apply (rule val.v_t_prim[where l = "(LU32 _)", simplified])
+   apply (clarsimp simp: wordarray_length_0_type_def \<xi>m_def val_wordarray_length_0_def)
+   apply (rule val.v_t_prim[where l = "(LU32 _)", simplified])
+  apply (clarsimp simp: wordarray_put2_0_type_def abbreviatedType5_def \<xi>m_def val_wordarray_put2_0_def)
+  apply (erule val.v_t_recordE)
+  apply (erule val.v_t_r_consE; clarsimp)
+   apply (erule val.v_t_abstractE)
+  apply (rule val.v_t_abstract)
+   apply (clarsimp simp: abs_typing_v_def)
+   apply (erule_tac x = i in allE; clarsimp)
+   apply (case_tac "i = unat idx")
+    apply (rule_tac x = val in exI; simp)
+   apply (rule_tac x = x in exI; simp)
+  apply simp
+  done
+
+lemma proc_env_u_v_matches_\<xi>0_\<xi>m_\<Xi>:
+  "proc_env_u_v_matches \<xi>0 \<xi>m \<Xi>"
+  apply (clarsimp simp: proc_env_u_v_matches_def)
+  apply (subst (asm) \<Xi>_def)
+  apply (subst (asm) assoc_lookup.simps)+
+  apply (clarsimp split: if_split_asm simp: \<xi>0_def)
+    apply (clarsimp simp: upd_wordarray_get_0_def wordarray_get_0_type_def abbreviatedType6_def)
+    apply (erule u_v_recE'; clarsimp)
+    apply (erule u_v_r_consE'; clarsimp)
+    apply (erule u_v_p_absE'; clarsimp)
+    apply (erule u_v_r_consE'; clarsimp)
+    apply (erule u_v_r_emptyE')
+    apply (erule u_v_primE')+
+    apply (subst (asm) lit_type.simps)+
+    apply clarsimp
+    apply (rule conjI)
+     apply (clarsimp simp: \<xi>m_def val_wordarray_get_0_def)
+     apply (rule_tac x = "{}" in exI)+
+     apply (clarsimp simp: abs_upd_val'_def frame_def word_less_nat_alt)
+     apply (erule_tac x = idx in allE)
+     apply clarsimp
+     apply (case_tac "unat idx < length xs"; clarsimp intro!: u_v_prim[where l = "(LU32 _)", simplified])
+    apply (clarsimp simp: word_less_nat_alt abs_upd_val'_def)
+    apply (case_tac a'; clarsimp simp: word_less_nat_alt)
+    apply (erule_tac x = idx in allE)
+    apply (case_tac "unat idx < length x1"; clarsimp)
+     apply (rule_tac x = "VPrim (LU32 x)" in exI)
+     apply (clarsimp simp: \<xi>m_def val_wordarray_get_0_def)
+    apply (rule_tac x = "VPrim (LU32 0)" in exI)
+    apply (clarsimp simp: \<xi>m_def val_wordarray_get_0_def)
+   apply (clarsimp simp: upd_wordarray_put2_0_def wordarray_put2_0_type_def abbreviatedType5_def)
+   apply (erule u_v_recE'; clarsimp)
+   apply (erule u_v_r_consE'; clarsimp)
+   apply (erule u_v_p_absE'; clarsimp)
+   apply (erule u_v_r_consE'; simp)
+   apply (erule conjE)+
+   apply (subst (asm) type_repr.simps[symmetric])+
+   apply clarsimp
+   apply (erule u_v_r_consE'; simp)
+   apply (erule conjE)+
+   apply (subst (asm) type_repr.simps[symmetric])+
+   apply clarsimp
+   apply (erule u_v_r_emptyE')
+   apply (erule u_v_primE')+
+   apply (subst (asm) lit_type.simps)+
+   apply clarsimp
+   apply (rule conjI)
+    apply (clarsimp simp: \<xi>m_def val_wordarray_put2_0_def)
+    apply (rule_tac x = ra in exI)
+    apply (rule_tac x = "insert p w" in exI)
+    apply clarsimp
+    apply (rule conjI)
+     apply (rule_tac a = a and  ptrl = undefined in u_v_p_abs_w[where ts = "[TPrim (Num U32)]", simplified])
+        apply simp
+       apply (clarsimp simp: abs_upd_val'_def)
+       apply (case_tac a; clarsimp)
+       apply (rule conjI)
+        apply (clarsimp simp: abs_typing_u_def)
+       apply (rule conjI)
+        apply (clarsimp simp: abs_typing_v_def word_less_nat_alt)
+        apply (erule_tac x = i in allE)
+        apply (case_tac "i = unat idx"; clarsimp)
+       apply (clarsimp simp: word_less_nat_alt)
+       apply (rule conjI)
+        apply (drule distinct_indices)
+        apply (clarsimp simp: word_less_nat_alt)
+        apply (erule_tac x = i in allE)+
+        apply clarsimp
+        apply (erule_tac x = idx in allE)
+        apply clarsimp
+       apply clarsimp
+       apply (erule_tac x = i in allE)
+       apply clarsimp
+       apply (case_tac "unat i = unat idx"; clarsimp)
+      apply (clarsimp simp: abs_upd_val'_def)
+      apply (erule_tac x = idx in allE)
+      apply clarsimp
+     apply simp
+    apply (clarsimp simp: frame_def)
+    apply (rule conjI; clarsimp)
+    apply (rule conjI)
+      apply (clarsimp simp: abs_upd_val'_def abs_typing_u_def)
+     apply (rule conjI; clarsimp)
+     apply (clarsimp simp: abs_upd_val'_def abs_typing_u_def)
+    apply (rule conjI; clarsimp)
+   apply (clarsimp simp: abs_upd_val'_def)
+   apply (case_tac a; clarsimp simp: abs_typing_u_def)
+   apply (case_tac a'; clarsimp)
+   apply (rule_tac x = "VAbstract (VWA (x1[unat idx := VPrim (LU32 val)]))" in exI)
+   apply (clarsimp simp: \<xi>m_def val_wordarray_put2_0_def)
+  apply (clarsimp simp: \<xi>0_def upd_wordarray_length_0_def wordarray_length_0_type_def)
+  apply (erule u_v_p_absE'; clarsimp)
+  apply (clarsimp simp: abs_upd_val'_def)
+  apply (case_tac a'a; clarsimp)
+  apply (rule conjI)
+   apply (clarsimp simp: \<xi>m_def val_wordarray_length_0_def)
+   apply (rule_tac x = "{}" in exI)+
+   apply (clarsimp simp: frame_def intro!: u_v_prim[where l = "(LU32 _)", simplified])
+  apply (clarsimp simp: abs_upd_val'_def)
+  apply (rule_tac x = "VPrim (LU32 len)" in exI)
+  apply (clarsimp simp: \<xi>m_def val_wordarray_length_0_def)
+  done
+
+lemma upd_proc_env_matches_ptrs_\<xi>0_\<Xi>:
+  "upd.proc_env_matches_ptrs \<xi>0 \<Xi>"
+  apply (unfold upd.proc_env_matches_ptrs_def)
+  apply clarsimp
+  apply (subst (asm) \<Xi>_def)
+  apply (subst (asm) assoc_lookup.simps)+
+  apply (clarsimp split: if_split_asm simp: \<xi>0_def)
+    apply (clarsimp simp: wordarray_get_0_type_def abbreviatedType6_def upd_wordarray_get_0_def)
+    apply (erule upd.u_t_recE; clarsimp)
+    apply (erule upd.u_t_r_consE; clarsimp)
+    apply (erule upd.u_t_p_absE; clarsimp)
+    apply (erule upd.u_t_r_consE; clarsimp)
+    apply (erule upd.u_t_r_emptyE; clarsimp)
+    apply (erule upd.u_t_primE; subst (asm) lit_type.simps; clarsimp)+
+    apply (rule_tac x = "{}" in exI)+
+    apply (clarsimp simp: frame_def abs_typing_u_def)
+    apply (erule_tac x = idx in allE)
+    apply (case_tac "idx < len"; clarsimp intro!: upd.u_t_prim[where l = "(LU32 _)", simplified])
+   apply (clarsimp simp: wordarray_put2_0_type_def abbreviatedType5_def upd_wordarray_put2_0_def)
+   apply (erule upd.u_t_recE; clarsimp)
+   apply (erule upd.u_t_r_consE; clarsimp)
+   apply (erule upd.u_t_p_absE; clarsimp)
+   apply (erule upd.u_t_r_consE; simp)
+   apply (erule conjE)+
+   apply (subst (asm) type_repr.simps[symmetric])+
+   apply clarsimp
+   apply (erule upd.u_t_r_consE; simp)
+   apply (erule conjE)+
+   apply (subst (asm) type_repr.simps[symmetric])+
+   apply clarsimp
+   apply (erule upd.u_t_r_emptyE)
+   apply (erule upd.u_t_primE)+
+   apply (subst (asm) lit_type.simps)+
+   apply clarsimp
+   apply (case_tac a; clarsimp)
+    apply (rule_tac x = ra in exI)
+    apply (rule_tac x = "insert p w" in exI)
+    apply (rule conjI)
+     apply (rename_tac len arr)
+     apply (rule_tac ptrl = undefined and a = "WAU32 len arr" in upd.u_t_p_abs_w[where ts = "[TPrim (Num U32)]", simplified])
+        apply simp
+       apply (clarsimp simp: abs_typing_u_def)
+      apply (clarsimp simp: abs_typing_u_def)
+     apply clarsimp
+    apply (clarsimp simp: frame_def abs_typing_u_def)
+    apply (rule conjI; clarsimp)
+     apply (rule conjI)
+      apply (rule disjI2)
+      apply (rule disjI2)
+      apply (rule_tac x = idx in exI; simp)
+     apply (rule conjI; clarsimp)
+    apply (rule conjI; clarsimp)
+   apply (clarsimp simp: abs_typing_u_def)
+  apply (clarsimp simp: wordarray_length_0_type_def upd_wordarray_length_0_def)
+  apply (erule upd.u_t_p_absE; clarsimp)
+  apply (rule_tac x = "{}" in exI)+
+  apply (clarsimp simp: frame_def intro!: upd.u_t_prim[where l = "(LU32 _)", simplified])
+  done
+
+lemma proc_ctx_wellformed_\<Xi>:
+  "proc_ctx_wellformed \<Xi>"
+  apply (clarsimp simp: proc_ctx_wellformed_def \<Xi>_def)
+  apply (clarsimp split: if_splits
+                  simp: assoc_lookup.simps
+                        wordarray_get_0_type_def abbreviatedType6_def wordarray_get_u32_type_def
+                        wordarray_length_0_type_def wordarray_length_u32_type_def
+                        wordarray_put2_0_type_def abbreviatedType5_def wordarray_put2_u32_type_def
+                        wordarray_fold_no_break_0_type_def abbreviatedType1_def
+                        wordarray_map_no_break_0_type_def abbreviatedType4_def abbreviatedType3_def abbreviatedType2_def
+                        dec_type_def dec_arr_type_def
+                        inc_type_def inc_arr_type_def
+                        sum_type_def sum_arr_type_def
+                        mul_type_def mul_arr_type_def)
+  done
+
+
+
 section "Correspondence From Isabelle Shallow Embedding to C"
 
 theorem shallow_C_wordarray_put2_corres:
@@ -306,7 +518,7 @@ theorem shallow_C_wordarray_put2_corres:
   apply clarsimp
   apply (frule val_rel_shallow_C_elim(3); clarsimp simp: val_rel_simp)
   apply (erule u_v_recE)
-  apply (erule u_v_r_consE; clarsimp simp: Generated_TypeProof.wordarray_put2_u32_type_def abbreviatedType1_def)
+  apply (erule u_v_r_consE; clarsimp simp: Generated_TypeProof.wordarray_put2_u32_type_def abbreviatedType5_def)
   apply (erule u_v_r_consE; clarsimp)+
   apply (erule u_v_r_emptyE; clarsimp)
   apply (erule u_v_primE)+
@@ -317,7 +529,7 @@ theorem shallow_C_wordarray_put2_corres:
   apply (erule u_sem_varE; clarsimp)
   apply (rule_tac x = "TCon ''WordArray'' [TPrim (Num U32)] (Boxed Writable undefined)" in exI)
   apply (rule_tac x = ra in exI)
-  apply (rule_tac x = "insert (ptr_val (arr_C uv\<^sub>C)) wa" in exI)
+  apply (rule_tac x = "insert (ptr_val (t2_C.arr_C uv\<^sub>C)) wa" in exI)
   apply (clarsimp simp: \<xi>0_def upd_wordarray_put2_0_def)
   apply (rule_tac ptrl = undefined and a = a in u_v_p_abs_w[where ts = "[TPrim (Num U32)]", simplified])
      apply simp
@@ -329,49 +541,24 @@ theorem shallow_C_wordarray_put2_corres:
      apply (clarsimp simp: abs_typing_v_def)
      apply (erule_tac x = i in allE)
      apply clarsimp
-     apply (case_tac "i = unat (idx_C uv\<^sub>C)"; clarsimp)
+     apply (case_tac "i = unat (t2_C.idx_C uv\<^sub>C)"; clarsimp)
     apply clarsimp
     apply (rule conjI; clarsimp)
      apply (drule distinct_indices)
      apply (erule_tac x = i in allE)+
      apply clarsimp
-     apply (erule_tac x = "idx_C uv\<^sub>C" in allE)
-     apply (cut_tac a = "idx_C uv\<^sub>C" and b = x11 in unat_mono; clarsimp)
+     apply (erule_tac x = "t2_C.idx_C uv\<^sub>C" in allE)
+     apply (clarsimp simp: word_less_nat_alt)
     apply (erule_tac x = i in allE)
     apply clarsimp
-    apply (case_tac "unat i = unat (idx_C uv\<^sub>C)"; clarsimp)
+    apply (case_tac "unat i = unat (t2_C.idx_C uv\<^sub>C)"; clarsimp)
    apply (clarsimp simp: abs_upd_val'_def)
-   apply (case_tac a; clarsimp simp: abs_typing_u_def)
+   apply (erule_tac x = " idx_C uv\<^sub>C" in allE)
+   apply clarsimp
   apply clarsimp
   done
 
 
-theorem shallow_C_wordarray_put2_corres':
-"\<lbrakk>\<And>i \<gamma> v' \<Gamma>' \<sigma> st.
-    \<lbrakk>i < length \<gamma>; val_rel (\<gamma> ! i) v'; \<Gamma>' ! i = option.Some (prod.fst (prod.snd wordarray_put2_0_type))\<rbrakk>
-    \<Longrightarrow> update_sem_init.corres abs_typing_u abs_repr_u (Generated.state_rel abs_repr_u) (App (AFun ''wordarray_put2_0'' []) (Var i))
-         (do x <- main_pp_inferred.wordarray_put2_0' v';
-             gets (\<lambda>s. x)
-          od)
-         \<xi>0 \<gamma>
-         (assoc_lookup
-           [(''wordarray_get_0'', wordarray_get_0_type), (''wordarray_length_0'', wordarray_length_0_type),
-            (''wordarray_put2_0'', wordarray_put2_0_type), (''wordarray_get_u32'', Generated_TypeProof.wordarray_get_u32_type),
-            (''wordarray_length_u32'', Generated_TypeProof.wordarray_length_u32_type),
-            (''wordarray_put2_u32'', Generated_TypeProof.wordarray_put2_u32_type)]
-           ([], TUnit, TUnit))
-         \<Gamma>' \<sigma> st;
- value_sem.rename_mono_prog abs_typing_v rename \<Xi> \<xi>m \<xi>p;
- vv\<^sub>m = value_sem.rename_val rename (value_sem.monoval vv\<^sub>p);
- correspondence_init.val_rel_shallow_C abs_repr_u abs_upd_val' rename vv\<^sub>s uv\<^sub>C vv\<^sub>p uv\<^sub>m \<xi>p \<sigma> \<Xi>; proc_ctx_wellformed \<Xi>;
- value_sem.proc_env_matches abs_typing_v \<xi>m \<Xi>;
- value_sem.matches abs_typing_v \<Xi> [vv\<^sub>m] [option.Some (prod.fst (prod.snd Generated_TypeProof.wordarray_put2_u32_type))]\<rbrakk>
-\<Longrightarrow> correspondence_init.corres_shallow_C abs_repr_u abs_typing_u abs_upd_val' rename (Generated.state_rel abs_repr_u)
-     (Generated_Shallow_Desugar.wordarray_put2_u32 vv\<^sub>s) Generated_TypeProof.wordarray_put2_u32
-     (main_pp_inferred.wordarray_put2_u32' uv\<^sub>C) \<xi>0 \<xi>m \<xi>p [uv\<^sub>m] [vv\<^sub>m] \<Xi>
-     [option.Some (prod.fst (prod.snd Generated_TypeProof.wordarray_put2_u32_type))] \<sigma> s"
-  apply (insert shallow_C_wordarray_put2_corres; force simp: \<Xi>_def)
-  done
 
 theorem shallow_C_wordarray_length_corres:
 "\<lbrakk>\<And>i \<gamma> v' \<Gamma>' \<sigma> st.
@@ -459,32 +646,6 @@ theorem shallow_C_wordarray_length_corres:
   apply (clarsimp simp: val_rel_simp)
   done
 
-theorem shallow_C_wordarray_length_corres':
-"\<lbrakk>\<And>i \<gamma> v' \<Gamma>' \<sigma> st.
-    \<lbrakk>i < length \<gamma>; val_rel (\<gamma> ! i) v'; \<Gamma>' ! i = option.Some (prod.fst (prod.snd wordarray_length_0_type))\<rbrakk>
-    \<Longrightarrow> update_sem_init.corres abs_typing_u abs_repr_u (Generated.state_rel abs_repr_u) (App (AFun ''wordarray_length_0'' []) (Var i))
-         (do x <- main_pp_inferred.wordarray_length_0' v';
-             gets (\<lambda>s. x)
-          od)
-         \<xi>0 \<gamma>
-         (assoc_lookup
-           [(''wordarray_get_0'', wordarray_get_0_type), (''wordarray_length_0'', wordarray_length_0_type),
-            (''wordarray_put2_0'', wordarray_put2_0_type), (''wordarray_get_u32'', Generated_TypeProof.wordarray_get_u32_type),
-            (''wordarray_length_u32'', Generated_TypeProof.wordarray_length_u32_type),
-            (''wordarray_put2_u32'', Generated_TypeProof.wordarray_put2_u32_type)]
-           ([], TUnit, TUnit))
-         \<Gamma>' \<sigma> st;
- value_sem.rename_mono_prog abs_typing_v rename \<Xi> \<xi>m \<xi>p;
- vv\<^sub>m = value_sem.rename_val rename (value_sem.monoval vv\<^sub>p);
- correspondence_init.val_rel_shallow_C abs_repr_u abs_upd_val' rename vv\<^sub>s uv\<^sub>C vv\<^sub>p uv\<^sub>m \<xi>p \<sigma> \<Xi>; proc_ctx_wellformed \<Xi>;
- value_sem.proc_env_matches abs_typing_v \<xi>m \<Xi>;
- value_sem.matches abs_typing_v \<Xi> [vv\<^sub>m] [option.Some (prod.fst (prod.snd Generated_TypeProof.wordarray_length_u32_type))]\<rbrakk>
-\<Longrightarrow> correspondence_init.corres_shallow_C abs_repr_u abs_typing_u abs_upd_val' rename (Generated.state_rel abs_repr_u)
-     (Generated_Shallow_Desugar.wordarray_length_u32 vv\<^sub>s) Generated_TypeProof.wordarray_length_u32
-     (main_pp_inferred.wordarray_length_u32' uv\<^sub>C) \<xi>0 \<xi>m \<xi>p [uv\<^sub>m] [vv\<^sub>m] \<Xi>
-     [option.Some (prod.fst (prod.snd Generated_TypeProof.wordarray_length_u32_type))] \<sigma> s"
-  apply (insert shallow_C_wordarray_length_corres; force simp: \<Xi>_def)
-  done
 
 theorem shallow_C_wordarray_get_corres:
 "\<lbrakk>\<And>i \<gamma> v' \<Gamma>' \<sigma> st.
@@ -546,7 +707,7 @@ theorem shallow_C_wordarray_get_corres:
                        in u_v_matches_proj_single'; simp)
   apply clarsimp
   apply (frule val_rel_shallow_C_elim(3))
-  apply (clarsimp simp: val_rel_simp wordarray_get_u32_type_def abbreviatedType2_def)
+  apply (clarsimp simp: val_rel_simp wordarray_get_u32_type_def abbreviatedType6_def)
   apply (erule u_v_recE)
   apply (erule u_v_r_consE; clarsimp)+
   apply (erule u_v_r_emptyE)
@@ -555,7 +716,6 @@ theorem shallow_C_wordarray_get_corres:
   apply (erule u_v_p_absE; clarsimp)
   apply (erule u_sem_appE; erule u_sem_afunE; clarsimp)
   apply (erule u_sem_varE; clarsimp simp: \<xi>0_def upd_wordarray_get_0_def)
-  apply (case_tac a; clarsimp simp: abs_upd_val'_def)
   apply (simp add: word_less_nat_alt)
   apply (rule conjI)
    apply (rule v_sem_let)
@@ -563,416 +723,15 @@ theorem shallow_C_wordarray_get_corres:
    apply (rule v_sem_abs_app)
      apply (rule v_sem_afun)
     apply (rule v_sem_var)
-   apply (clarsimp simp: \<xi>m_def val_wordarray_get_0_def)
+   apply (clarsimp simp: \<xi>m_def val_wordarray_get_0_def abs_upd_val'_def)
+  apply (erule_tac x = "t1_C.p2_C uv\<^sub>C" in allE; clarsimp simp: word_less_nat_alt)
   apply (subst val_rel_shallow_C_def)
   apply (rule_tac x = "TPrim (Num U32)" in exI)
   apply (rule_tac x = "{}" in exI)+
-  apply (clarsimp simp: Generated_Shallow_Desugar.wordarray_get_u32_def wordarray_get')
-  apply (erule_tac x = "unat (p2_C uv\<^sub>C)" in allE)
+  apply (clarsimp simp: Generated_Shallow_Desugar.wordarray_get_u32_def wordarray_get' abs_upd_val'_def word_less_nat_alt)
+  apply (erule_tac x = "unat (t1_C.p2_C uv\<^sub>C)" in allE)
   apply (force simp: val_rel_simp intro!: u_v_prim[where l = "LU32 _", simplified])
   done
-
-theorem shallow_C_wordarray_get_corres':
-"\<lbrakk>\<And>i \<gamma> v' \<Gamma>' \<sigma> st.
-    \<lbrakk>i < length \<gamma>; val_rel (\<gamma> ! i) v'; \<Gamma>' ! i = option.Some (prod.fst (prod.snd wordarray_get_0_type))\<rbrakk>
-    \<Longrightarrow> update_sem_init.corres abs_typing_u abs_repr_u (Generated.state_rel abs_repr_u) (App (AFun ''wordarray_get_0'' []) (Var i))
-         (do x <- main_pp_inferred.wordarray_get_0' v';
-             gets (\<lambda>s. x)
-          od)
-         \<xi>0 \<gamma> 
-           (assoc_lookup
-           [(''wordarray_get_0'', wordarray_get_0_type), (''wordarray_length_0'', wordarray_length_0_type),
-            (''wordarray_put2_0'', wordarray_put2_0_type), (''wordarray_get_u32'', Generated_TypeProof.wordarray_get_u32_type),
-            (''wordarray_length_u32'', Generated_TypeProof.wordarray_length_u32_type),
-            (''wordarray_put2_u32'', Generated_TypeProof.wordarray_put2_u32_type)]
-           ([], TUnit, TUnit)) \<Gamma>' \<sigma> st;
- value_sem.rename_mono_prog abs_typing_v rename \<Xi> \<xi>m \<xi>p; vv\<^sub>m = value_sem.rename_val rename (value_sem.monoval vv\<^sub>p);
- correspondence_init.val_rel_shallow_C abs_repr_u abs_upd_val' rename vv\<^sub>s uv\<^sub>C vv\<^sub>p uv\<^sub>m \<xi>p \<sigma> \<Xi>; proc_ctx_wellformed \<Xi>;
- value_sem.proc_env_matches abs_typing_v \<xi>m \<Xi>;
- value_sem.matches abs_typing_v \<Xi> [vv\<^sub>m] [option.Some (prod.fst (prod.snd Generated_TypeProof.wordarray_get_u32_type))]\<rbrakk>
-\<Longrightarrow> correspondence_init.corres_shallow_C abs_repr_u abs_typing_u abs_upd_val' rename (Generated.state_rel abs_repr_u)
-     (Generated_Shallow_Desugar.wordarray_get_u32 vv\<^sub>s) Generated_TypeProof.wordarray_get_u32
-     (main_pp_inferred.wordarray_get_u32' uv\<^sub>C) \<xi>0 \<xi>m \<xi>p [uv\<^sub>m] [vv\<^sub>m] \<Xi>
-     [option.Some (prod.fst (prod.snd Generated_TypeProof.wordarray_get_u32_type))] \<sigma> s"
-  apply (insert shallow_C_wordarray_get_corres; force simp: \<Xi>_def)
-  done
-
-
-section "Naturally True Shared Assumptions for Isabelle to C Correspondence Lemmas"
-
-lemma value_sem_rename_mono_prog_rename_\<Xi>_\<xi>m_\<xi>p: 
-  "value_sem.rename_mono_prog abs_typing_v rename \<Xi> \<xi>m \<xi>p"
-  apply (clarsimp simp: val.rename_mono_prog_def)
-  apply (rule_tac x = v' in exI)
-  apply (rule conjI)
-   apply (clarsimp simp: rename_def \<xi>m_def)
-   apply (case_tac "ts = [TPrim (Num U32)]"; clarsimp)
-   apply (case_tac "f =''wordarray_put2''")
-    apply (clarsimp simp: val_wordarray_put2_0_def)
-    apply (case_tac v; clarsimp)
-    apply (case_tac x4; clarsimp)
-    apply (case_tac a; clarsimp)
-    apply (case_tac x5; clarsimp)
-    apply (case_tac list; clarsimp)
-    apply (case_tac a; clarsimp)
-    apply (case_tac x1a; clarsimp)
-    apply (case_tac lista; clarsimp)
-    apply (case_tac a; clarsimp)
-    apply (case_tac x1a; clarsimp)
-    apply (case_tac list; clarsimp)
-   apply (case_tac "f =''wordarray_length''")
-    apply (clarsimp simp: val_wordarray_length_0_def)
-    apply (case_tac v; clarsimp)
-    apply (case_tac x5; clarsimp)
-    apply (case_tac v'; clarsimp)
-   apply (case_tac "f =''wordarray_get''")
-    apply (clarsimp simp: val_wordarray_get_0_def)
-    apply (case_tac v; clarsimp)
-    apply (case_tac x4; clarsimp)
-    apply (case_tac a; clarsimp)
-    apply (case_tac x5; clarsimp)
-    apply (case_tac list; clarsimp)
-    apply (case_tac a; clarsimp)
-    apply (case_tac x1a; clarsimp)
-    apply (case_tac lista; clarsimp)
-    apply (clarsimp split: if_split_asm)
-   apply clarsimp
-  apply (clarsimp simp: \<xi>m_def \<xi>p_def)
-  apply (clarsimp simp: rename_def)
-  apply (case_tac "ts = [TPrim (Num U32)]"; clarsimp)
-  apply (rule conjI; clarsimp)
-   apply (clarsimp simp: val_wordarray_length_0_def)
-   apply (case_tac v; clarsimp)
-  apply (rule conjI; clarsimp)
-   apply (clarsimp simp: val_wordarray_get_0_def)
-   apply (case_tac v; clarsimp)
-   apply (case_tac x4; clarsimp)
-   apply (case_tac a; clarsimp)
-   apply (case_tac x5; clarsimp)
-   apply (case_tac list; clarsimp)
-   apply (case_tac a; clarsimp)
-   apply (case_tac x1a; clarsimp)
-   apply (case_tac lista; clarsimp)
-  apply (rule conjI)
-   apply (clarsimp simp: val_wordarray_put2_0_def)
-   apply (case_tac v; clarsimp)
-   apply (case_tac x4; clarsimp)
-   apply (case_tac a; clarsimp)
-   apply (case_tac x5; clarsimp)
-   apply (case_tac list; clarsimp)
-   apply (case_tac a; clarsimp)
-   apply (case_tac x1a; clarsimp)
-   apply (case_tac lista; clarsimp)
-   apply (case_tac a; clarsimp)
-   apply (case_tac x1a; clarsimp)
-   apply (case_tac list; clarsimp)
-  apply (case_tac "f = ''wordarray_put2''"; clarsimp)
-  done
-
-lemma val_proc_env_matches_\<xi>m_\<Xi>:
-  "val.proc_env_matches \<xi>m \<Xi>"
-  apply (clarsimp simp: val.proc_env_matches_def \<Xi>_def)
-  apply (case_tac "f = ''wordarray_put2_0''")
-   apply (clarsimp simp: wordarray_put2_0_type_def abbreviatedType1_def \<xi>m_def val_wordarray_put2_0_def)
-   apply (case_tac v; clarsimp)
-   apply (case_tac x4; clarsimp)
-   apply (case_tac a; clarsimp)
-   apply (case_tac x5; clarsimp)
-   apply (case_tac list; clarsimp)
-   apply (case_tac a; clarsimp)
-   apply (case_tac x1a; clarsimp)
-   apply (case_tac lista; clarsimp)
-   apply (case_tac a; clarsimp)
-   apply (case_tac x1a; clarsimp)
-   apply (case_tac list; clarsimp)
-   apply (erule val.v_t_recordE)
-   apply (erule val.v_t_r_consE; clarsimp)
-   apply (rule val.v_t_abstract)
-    apply (erule val.v_t_abstractE)
-    apply (clarsimp simp: abs_typing_v_def)
-    apply (erule_tac x = i in allE; clarsimp)
-    apply (case_tac "i = unat x4")
-     apply (rule_tac x = x4a in exI; simp)
-    apply (rule_tac x = x in exI; simp)
-   apply simp
-  apply (case_tac "f = ''wordarray_put2_u32''")
-   apply (clarsimp simp: \<xi>m_def)
-  apply (case_tac "f = ''wordarray_get_0''")
-   apply (clarsimp simp: wordarray_get_0_type_def abbreviatedType2_def \<xi>m_def val_wordarray_get_0_def)
-   apply (case_tac v; clarsimp)
-   apply (case_tac x4; clarsimp)
-   apply (case_tac a; clarsimp)
-   apply (case_tac x5; clarsimp)
-   apply (case_tac list; clarsimp)
-   apply (case_tac a; clarsimp)
-   apply (case_tac x1a; clarsimp)
-   apply (case_tac lista; clarsimp)
-   apply (clarsimp split: if_split_asm intro!: val.v_t_prim[where l = "(LU32 _)", simplified])
-  apply (case_tac "f = ''wordarray_get_u32''")
-   apply (clarsimp simp: \<xi>m_def)
-  apply (case_tac "f = ''wordarray_length_0''")
-   apply (clarsimp simp: wordarray_length_0_type_def \<xi>m_def val_wordarray_length_0_def)
-   apply (case_tac v; clarsimp)
-   apply (case_tac x5; clarsimp)
-   apply (case_tac v'; clarsimp)
-   apply (case_tac x1a; clarsimp)
-   apply (rule val.v_t_prim[where l = "(LU32 _)", simplified])
-  apply (case_tac "f = ''wordarray_length_u32''")
-   apply (clarsimp simp: \<xi>m_def)
-  apply (clarsimp simp: \<xi>m_def)
-  done
-
-lemma proc_env_u_v_matches_\<xi>0_\<xi>m_\<Xi>:
-  "proc_env_u_v_matches \<xi>0 \<xi>m \<Xi>"
-  apply (clarsimp simp: proc_env_u_v_matches_def)
-  apply (clarsimp simp: \<Xi>_def)
-  apply (case_tac "f = ''wordarray_put2_u32''")
-   apply (clarsimp simp: \<xi>0_def)
-  apply (case_tac "f = ''wordarray_get_u32''")
-   apply (clarsimp simp: \<xi>0_def)
-  apply (case_tac "f = ''wordarray_length_u32''")
-   apply (clarsimp simp: \<xi>0_def)
-  apply (case_tac "f = ''wordarray_length_0''")
-   apply (clarsimp simp: \<xi>0_def upd_wordarray_length_0_def)
-  apply (case_tac aa; clarsimp)
-  apply (case_tac "\<sigma>' x91"; clarsimp)
-  apply (case_tac aa; clarsimp)
-   apply (case_tac x5; clarsimp)
-   apply (clarsimp simp: wordarray_length_0_type_def)
-   apply (erule u_v_p_absE'; clarsimp)
-   apply (clarsimp simp: abs_upd_val'_def)
-    apply (case_tac a'a; clarsimp)
-   apply (rule conjI)
-    apply (clarsimp simp: \<xi>m_def val_wordarray_length_0_def)
-    apply (case_tac v'; clarsimp)
-    apply (case_tac x1a; clarsimp)
-    apply (rule_tac x = "{}" in exI)+
-    apply (clarsimp simp: frame_def intro!: u_v_prim[where l = "(LU32 _)", simplified])
-   apply (clarsimp simp: abs_upd_val'_def)
-   apply (rule_tac x = "VPrim (LU32 x11)" in exI)
-   apply (clarsimp simp: \<xi>m_def val_wordarray_length_0_def)
-  apply (case_tac "f = ''wordarray_put2_0''")
-   apply (clarsimp simp: \<xi>0_def upd_wordarray_put2_0_def)
-   apply (case_tac aa; clarsimp)
-   apply (case_tac x4; clarsimp)
-   apply (case_tac aa; clarsimp)
-   apply (case_tac list; clarsimp)
-   apply (case_tac aa; clarsimp)
-   apply (case_tac x1; clarsimp)
-   apply (case_tac lista; clarsimp)
-   apply (case_tac aa; clarsimp)
-   apply (case_tac x1; clarsimp)
-   apply (case_tac list; clarsimp)
-   apply (clarsimp simp: wordarray_put2_0_type_def abbreviatedType1_def)
-   apply (erule u_v_recE')
-   apply clarsimp
-   apply (erule u_v_r_consE'; clarsimp)+
-   apply (erule u_v_r_emptyE')
-   apply clarsimp
-   apply (erule u_v_primE')+
-   apply (subst (asm) lit_type.simps)+
-   apply clarsimp
-   apply (erule u_v_p_absE'; clarsimp)
-   apply (rule conjI)
-    apply (clarsimp simp: \<xi>m_def val_wordarray_put2_0_def)
-    apply (case_tac a'; clarsimp)
-    apply (rule_tac x = ra in exI)
-    apply (rule_tac x = "insert x91 w" in exI)
-    apply clarsimp
-    apply (rule conjI)
-     apply (rule_tac a = a and  ptrl = undefined in u_v_p_abs_w[where ts = "[TPrim (Num U32)]", simplified])
-        apply simp
-       apply (clarsimp simp: abs_upd_val'_def)
-       apply (case_tac a; clarsimp)
-       apply (rule conjI)
-        apply (clarsimp simp: abs_typing_u_def)
-       apply (rule conjI)
-        apply (clarsimp simp: abs_typing_v_def)
-        apply (erule_tac x = i in allE)
-        apply (case_tac "i = unat x4"; clarsimp)
-       apply clarsimp
-       apply (rule conjI)
-        apply clarsimp
-        apply (drule distinct_indices)
-        apply (erule_tac x = i in allE)+
-        apply clarsimp
-        apply (erule_tac x = x4 in allE)
-        apply clarsimp
-        apply (cut_tac a = x4 and b = x11 in unat_mono; simp)
-       apply clarsimp
-       apply (erule_tac x = i in allE)
-       apply clarsimp
-       apply (case_tac "unat i = unat x4"; clarsimp)
-      apply (clarsimp simp: abs_upd_val'_def)
-      apply (case_tac a;  clarsimp)
-      apply (erule_tac x = x4 in allE)
-      apply clarsimp
-     apply simp
-    apply (clarsimp simp: frame_def)
-    apply (rule conjI)
-     apply clarsimp
-    apply (rule conjI; clarsimp)
-    apply (clarsimp simp: abs_upd_val'_def abs_typing_u_def)
-    apply (case_tac a; clarsimp)
-   apply (clarsimp simp: abs_upd_val'_def)
-   apply (case_tac a; clarsimp simp: abs_typing_u_def)
-   apply (case_tac a'; clarsimp)
-   apply (rule_tac x = "VAbstract (VWA (x1[unat x4 := VPrim (LU32 x4a)]))" in exI)
-   apply (clarsimp simp: \<xi>m_def val_wordarray_put2_0_def)
-  apply (case_tac "f = ''wordarray_get_0''")
-   apply (clarsimp simp: \<xi>0_def upd_wordarray_get_0_def)
-   apply (case_tac aa; clarsimp)
-   apply (case_tac x4; clarsimp)
-   apply (case_tac aa; clarsimp)
-   apply (case_tac list; clarsimp)
-   apply (case_tac aa; clarsimp)
-   apply (case_tac x1; clarsimp)
-   apply (case_tac lista; clarsimp)
-   apply (case_tac "\<sigma>' x91"; clarsimp)
-   apply (case_tac aa; clarsimp)
-   apply (case_tac x5; clarsimp)
-   apply (clarsimp simp: wordarray_get_0_type_def abbreviatedType2_def)
-   apply (erule u_v_recE')
-   apply clarsimp
-   apply (erule u_v_r_consE'; clarsimp)+
-   apply (erule u_v_r_emptyE')
-   apply clarsimp
-   apply (erule u_v_primE')+
-   apply (subst (asm) lit_type.simps)+
-   apply clarsimp
-   apply (erule u_v_p_absE'; clarsimp)
-   apply (rule conjI)
-    apply (clarsimp simp: \<xi>m_def val_wordarray_get_0_def)
-    apply (case_tac a'; clarsimp)
-    apply (rule_tac x = "{}" in exI)+
-    apply (clarsimp simp: abs_upd_val'_def frame_def)
-    apply (erule_tac x = x4 in allE)
-    apply (clarsimp split: if_split_asm)
-     apply (cut_tac a = x4 and b = x11 in unat_mono; simp)
-     apply (clarsimp intro!:  u_v_prim[where l = "(LU32 _)", simplified])
-    apply (subgoal_tac "\<not> unat x4 < length x1"; 
-            clarsimp simp: word_less_nat_alt intro!: u_v_prim[where l = "(LU32 _)", simplified])
-   apply (clarsimp simp: abs_upd_val'_def)
-   apply (case_tac a'; clarsimp)
-   apply (erule_tac x = x4 in allE)
-   apply (case_tac "x4 < x11"; clarsimp)
-    apply (rule_tac x = "VPrim (LU32 x)" in exI)
-    apply (clarsimp simp: \<xi>m_def val_wordarray_get_0_def)
-    apply (cut_tac a = x4 and b = x11 in unat_mono; fastforce)
-   apply (rule_tac x = "VPrim (LU32 0)" in exI)
-   apply (clarsimp simp: \<xi>m_def val_wordarray_get_0_def word_less_nat_alt)
-  apply (clarsimp simp: \<xi>0_def)
-  done
-
-lemma upd_proc_env_matches_ptrs_\<xi>0_\<Xi>:
-  "upd.proc_env_matches_ptrs \<xi>0 \<Xi>"
-  apply (unfold upd.proc_env_matches_ptrs_def)
-  apply clarsimp
-  apply (subst (asm) \<Xi>_def)
-  apply (case_tac  "f = ''wordarray_put2_0''")
-   apply clarsimp
-   apply (clarsimp simp: wordarray_put2_0_type_def abbreviatedType1_def)
-   apply (clarsimp simp:  \<Xi>_def)
-   apply (case_tac v; clarsimp simp: \<xi>0_def upd_wordarray_put2_0_def)
-   apply (case_tac x4; clarsimp)
-   apply (case_tac a; clarsimp)
-   apply (case_tac list; clarsimp)
-   apply (case_tac a; clarsimp)
-   apply (case_tac x1; clarsimp)
-   apply (case_tac lista; clarsimp)
-   apply (case_tac a; clarsimp)
-   apply (case_tac x1; clarsimp)
-   apply (case_tac list; clarsimp)
-   apply (erule upd.u_t_recE; clarsimp)
-   apply (erule upd.u_t_r_consE; clarsimp)+
-   apply (erule upd.u_t_p_absE; clarsimp)
-   apply (erule upd.u_t_primE)+
-   apply (subst (asm) lit_type.simps)+
-   apply (erule upd.u_t_r_emptyE)
-   apply clarsimp
-   apply (rename_tac p i v r av w)
-   apply (case_tac av; clarsimp)
-   apply (rule_tac x = r in exI)
-    apply (rule_tac x = "insert p w" in exI)
-    apply (rule conjI)
-     apply (rename_tac len arr)
-     apply (rule_tac ptrl = undefined and a = "WAU32 len arr" in upd.u_t_p_abs_w[where ts = "[TPrim (Num U32)]", simplified])
-        apply simp
-       apply (clarsimp simp: abs_typing_u_def)
-      apply (clarsimp simp: abs_typing_u_def)
-     apply clarsimp
-    apply (clarsimp simp: frame_def abs_typing_u_def)
-    apply (rule conjI; clarsimp)
-     apply (rule conjI)
-      apply (rule disjI2)
-      apply (rule disjI2)
-      apply (rule_tac x = i in exI; simp)
-     apply (rule conjI; clarsimp)
-    apply (rule conjI; clarsimp)
-   apply (clarsimp simp: abs_typing_u_def)
-  apply (case_tac  "f = ''wordarray_put2_u32''")
-   apply (clarsimp simp: wordarray_put2_u32_type_def abbreviatedType1_def \<xi>0_def)
-  apply (case_tac  "f = ''wordarray_get_0''")
-   apply clarsimp
-   apply (clarsimp simp: wordarray_get_0_type_def abbreviatedType2_def)
-   apply (clarsimp simp:  \<Xi>_def)
-   apply (case_tac v; clarsimp simp: \<xi>0_def upd_wordarray_get_0_def)
-   apply (case_tac x4; clarsimp)
-   apply (case_tac a; clarsimp)
-   apply (case_tac list; clarsimp)
-   apply (case_tac a; clarsimp)
-   apply (case_tac x1; clarsimp)
-   apply (case_tac lista; clarsimp)
-   apply (erule upd.u_t_recE; clarsimp)
-   apply (erule upd.u_t_r_consE; clarsimp)+
-   apply (erule upd.u_t_p_absE; clarsimp)
-   apply (erule upd.u_t_primE)+
-   apply (subst (asm) lit_type.simps)+
-   apply (erule upd.u_t_r_emptyE)
-   apply clarsimp
-   apply (rule_tac x = "{}" in exI)+
-   apply (clarsimp simp: frame_def)
-   apply (clarsimp simp: abs_typing_u_def)
-   apply (case_tac a;  clarsimp)
-   apply (erule_tac x = x4 in allE)
-   apply (clarsimp split: if_split_asm intro!: upd.u_t_prim[where l = "(LU32 _)", simplified])
-  apply (case_tac  "f = ''wordarray_get_u32''")
-   apply (clarsimp simp: wordarray_get_u32_type_def abbreviatedType2_def \<xi>0_def)
-  apply (case_tac  "f = ''wordarray_length_0''")
-   apply clarsimp
-   apply (clarsimp simp: wordarray_length_0_type_def)
-   apply (clarsimp simp:  \<Xi>_def)
-   apply (case_tac v; clarsimp simp: \<xi>0_def upd_wordarray_length_0_def)
-   apply (case_tac "\<sigma>' x91"; clarsimp)
-   apply (case_tac a; clarsimp)
-   apply (case_tac x5; clarsimp)
-   apply (erule upd.u_t_p_absE; clarsimp)
-   apply (rule_tac x = "{}" in exI)+
-   apply (clarsimp simp: frame_def intro!: upd.u_t_prim[where l = "(LU32 _)", simplified])
-  apply (case_tac  "f = ''wordarray_length_u32''")
-   apply (clarsimp simp: wordarray_length_u32_type_def \<xi>0_def)
-  apply (clarsimp simp: \<xi>0_def)
-  done
-
-
-lemma proc_ctx_wellformed_\<Xi>:
-  "proc_ctx_wellformed \<Xi>"
-  apply (clarsimp simp: proc_ctx_wellformed_def \<Xi>_def)
-  apply (case_tac "f = ''wordarray_put2_0''")
-   apply (clarsimp simp: wordarray_put2_0_type_def abbreviatedType1_def)
-  apply (case_tac "f = ''wordarray_put2_u32''")
-   apply (clarsimp simp: wordarray_put2_u32_type_def abbreviatedType1_def)
-  apply (case_tac "f = ''wordarray_get_0''")
-   apply (clarsimp simp: wordarray_get_0_type_def abbreviatedType2_def)
-  apply (case_tac "f = ''wordarray_get_u32''")
-   apply (clarsimp simp: wordarray_get_u32_type_def abbreviatedType2_def)
-  apply (case_tac "f = ''wordarray_length_0''")
-   apply (clarsimp simp: wordarray_length_0_type_def)
-  apply (case_tac "f = ''wordarray_length_u32''")
-   apply (clarsimp simp: wordarray_length_u32_type_def)
-  apply clarsimp
-  done
-
 
 section "Correspondence Lemmas Between Update Semantics and C"
 
@@ -989,7 +748,7 @@ lemma upd_C_wordarray_put2_corres:
   apply (thin_tac "i < length \<gamma>")
   apply (thin_tac "val_rel (\<gamma> ! i) v'")
   apply (thin_tac "\<Gamma>' ! i = option.Some (prod.fst (prod.snd (\<Xi> ''wordarray_put2_0'')))")
-  apply (clarsimp simp: val_rel_simp \<Xi>_def wordarray_put2_0_type_def abbreviatedType1_def)
+  apply (clarsimp simp: val_rel_simp \<Xi>_def wordarray_put2_0_type_def abbreviatedType5_def)
   apply (erule upd.u_t_recE)
   apply (erule upd.u_t_r_consE; clarsimp)+
   apply (erule upd.u_t_primE)+
@@ -1001,18 +760,16 @@ lemma upd_C_wordarray_put2_corres:
   apply (rule conjI)
    apply (monad_eq simp: wordarray_put2_0'_def)
    apply (clarsimp simp: state_rel_def heap_rel_def)
-   apply (erule_tac x = "arr_C x'" in allE)
-   apply (erule_tac x = "values_C (heap_WordArray_u32_C st (arr_C x')) +\<^sub>p uint (idx_C x')" in allE)
+   apply (erule_tac x = "t2_C.arr_C x'" in allE)
+   apply (erule_tac x = "values_C (heap_WordArray_u32_C st (t2_C.arr_C x')) +\<^sub>p uint (t2_C.idx_C x')" in allE)
    apply (clarsimp simp: heap_rel_ptr_def heap_rel_ptr_w32_def abs_repr_u_def is_valid_simp type_rel_simp)
-   apply (erule_tac x = "idx_C x'" in allE)+
+   apply (erule_tac x = "t2_C.idx_C x'" in allE)+
    apply (clarsimp simp: val_rel_simp heap_simp type_rel_simp)
   apply clarsimp
-  apply (rule_tac x = "\<lambda>l. (case (\<sigma> \<circ> ptr_val \<circ> arr_C) x' of 
-                                option.Some (UAbstract (WAU32 len arr)) \<Rightarrow>
-                                      (if l = arr + 4 * idx_C x' \<and> idx_C x' < len 
-                                          then option.Some (UPrim (LU32 (val_C x'))) 
-                                      else \<sigma> l)
-                              | _  \<Rightarrow> \<sigma> l)" in exI)
+  apply (rule_tac x = "\<lambda>l. (if \<exists>len arr. (\<sigma> \<circ> ptr_val \<circ> t2_C.arr_C) x' = option.Some (UAbstract (WAU32 len arr)) \<and> 
+                                l = arr + 4 * t2_C.idx_C x' \<and> t2_C.idx_C x' < len 
+                            then option.Some (UPrim (LU32 (t2_C.val_C x'))) 
+                            else \<sigma> l)" in exI)
   apply (rule_tac x = "UPtr (ptr_val y') (RCon ''WordArray'' [RPrim (Num U32)])" in exI)
   apply (rule conjI)
    apply (monad_eq simp: wordarray_put2_0'_def \<xi>0_def upd_wordarray_put2_0_def)
@@ -1024,40 +781,22 @@ lemma upd_C_wordarray_put2_corres:
    apply (rule conjI; clarsimp)
     apply (clarsimp simp: type_rel_simp)
    apply (monad_eq simp: wordarray_put2_0'_def)
-   apply (case_tac "idx_C x' < SCAST(32 signed \<rightarrow> 32) (len_C (heap_WordArray_u32_C st (arr_C x')))"; 
+   apply (case_tac "idx_C x' < SCAST(32 signed \<rightarrow> 32) (len_C (heap_WordArray_u32_C st (t2_C.arr_C x')))"; 
           drule_tac p = x and uv = uv in all_heap_rel_ptrD; clarsimp simp: is_valid_simp heap_simp)
-  apply (erule_tac x = "arr_C x'" in allE)
+  apply (erule_tac x = "t2_C.arr_C x'" in allE)
   apply (clarsimp simp: heap_rel_meta_def abs_repr_u_def type_rel_simp val_rel_simp)
   apply (monad_eq simp: wordarray_put2_0'_def heap_simp is_valid_simp)
   apply (rule conjI; clarsimp)
-   apply (drule_tac p = "values_C (heap_WordArray_u32_C st (arr_C x')) +\<^sub>p uint (idx_C x')" and 
+   apply (drule_tac p = "values_C (heap_WordArray_u32_C st (t2_C.arr_C x')) +\<^sub>p uint (t2_C.idx_C x')" and 
                    uv = uv in all_heap_rel_ptrD; clarsimp simp: type_rel_simp val_rel_simp)
   apply (rule conjI)
    apply (clarsimp simp: ptr_add_def)
    apply (metis Ptr_ptr_val mult.commute)
   apply clarsimp
-  apply (case_tac "idx_C x' < SCAST(32 signed \<rightarrow> 32) (len_C (heap_WordArray_u32_C st (arr_C x')))";
+  apply (case_tac "idx_C x' < SCAST(32 signed \<rightarrow> 32) (len_C (heap_WordArray_u32_C st (t2_C.arr_C x')))";
          drule_tac p = x and uv = uv in all_heap_rel_ptrD; clarsimp simp: type_rel_simp val_rel_simp)
   done
 
-lemma upd_C_wordarray_put2_corres':
-  "\<And>i \<gamma> v' \<Gamma>' \<sigma> st.
-    \<lbrakk>i < length \<gamma>; val_rel (\<gamma> ! i) v'; \<Gamma>' ! i = option.Some (prod.fst (prod.snd wordarray_put2_0_type))\<rbrakk>
-    \<Longrightarrow> update_sem_init.corres abs_typing_u abs_repr_u (Generated.state_rel abs_repr_u) (App (AFun ''wordarray_put2_0'' []) (Var i))
-         (do x <- main_pp_inferred.wordarray_put2_0' v';
-             gets (\<lambda>s. x)
-          od)
-         \<xi>0 \<gamma>
-         (assoc_lookup
-           [(''wordarray_get_0'', wordarray_get_0_type), (''wordarray_length_0'', wordarray_length_0_type),
-            (''wordarray_put2_0'', wordarray_put2_0_type), (''wordarray_get_u32'', Generated_TypeProof.wordarray_get_u32_type),
-            (''wordarray_length_u32'', Generated_TypeProof.wordarray_length_u32_type),
-            (''wordarray_put2_u32'', Generated_TypeProof.wordarray_put2_u32_type)]
-           ([], TUnit, TUnit))
-         \<Gamma>' \<sigma> st"
-  apply (insert upd_C_wordarray_put2_corres)
-  apply (force simp: \<Xi>_def)
-  done
 
 lemma upd_C_wordarray_length_corres:
 "\<And>i \<gamma> v' \<Gamma>' \<sigma> st.
@@ -1092,25 +831,6 @@ lemma upd_C_wordarray_length_corres:
   done
 
 
-lemma upd_C_wordarray_length_corres':
-"\<And>i \<gamma> v' \<Gamma>' \<sigma> st.
-    \<lbrakk>i < length \<gamma>; val_rel (\<gamma> ! i) v'; \<Gamma>' ! i = option.Some (prod.fst (prod.snd wordarray_length_0_type))\<rbrakk>
-    \<Longrightarrow> update_sem_init.corres abs_typing_u abs_repr_u (Generated.state_rel abs_repr_u) (App (AFun ''wordarray_length_0'' []) (Var i))
-         (do x <- main_pp_inferred.wordarray_length_0' v';
-             gets (\<lambda>s. x)
-          od)
-         \<xi>0 \<gamma>
-         (assoc_lookup
-           [(''wordarray_get_0'', wordarray_get_0_type), (''wordarray_length_0'', wordarray_length_0_type),
-            (''wordarray_put2_0'', wordarray_put2_0_type), (''wordarray_get_u32'', Generated_TypeProof.wordarray_get_u32_type),
-            (''wordarray_length_u32'', Generated_TypeProof.wordarray_length_u32_type),
-            (''wordarray_put2_u32'', Generated_TypeProof.wordarray_put2_u32_type)]
-           ([], TUnit, TUnit))
-         \<Gamma>' \<sigma> st"
-  apply (insert upd_C_wordarray_length_corres)
-  apply (force simp: \<Xi>_def)
-  done
-
 lemma upd_C_wordarray_get_corres:
 "\<And>i \<gamma> v' \<Gamma>' \<sigma> st.
     \<lbrakk>i < length \<gamma>; val_rel (\<gamma> ! i) v'; \<Gamma>' ! i = option.Some (prod.fst (prod.snd (\<Xi> ''wordarray_get_0'')))\<rbrakk>
@@ -1124,7 +844,7 @@ lemma upd_C_wordarray_get_corres:
   apply (thin_tac "i < length \<gamma>")
   apply (thin_tac "val_rel (\<gamma> ! i) v'")
   apply (thin_tac "\<Gamma>' ! i = option.Some (prod.fst (prod.snd (\<Xi> ''wordarray_get_0'')))")
-  apply (clarsimp simp: val_rel_simp \<Xi>_def wordarray_get_0_type_def abbreviatedType2_def)
+  apply (clarsimp simp: val_rel_simp \<Xi>_def wordarray_get_0_type_def abbreviatedType6_def)
   apply (erule upd.u_t_recE)
   apply (erule upd.u_t_r_consE; clarsimp)+
   apply (erule upd.u_t_r_emptyE)
@@ -1134,45 +854,26 @@ lemma upd_C_wordarray_get_corres:
   apply (rule conjI)
    apply (monad_eq simp: wordarray_get_0'_def)
    apply (clarsimp simp: state_rel_def heap_rel_def heap_rel_ptr_meta heap_rel_ptr_w32_meta)
-   apply (drule_tac p = "p1_C x'" and uv = "UAbstract (WAU32 x11 x12)" in all_heap_rel_ptrD; 
+   apply (drule_tac p = "t1_C.p1_C x'" and uv = "UAbstract (WAU32 x11 x12)" in all_heap_rel_ptrD; 
           clarsimp simp: type_rel_simp abs_repr_u_def val_rel_simp is_valid_simp heap_simp)
    apply (drule not_le_imp_less)
-   apply (erule_tac x = "p2_C x'" in allE; clarsimp)
-   apply (drule_tac p = "values_C (heap_WordArray_u32_C st (p1_C x')) +\<^sub>p uint (p2_C x')" and
+   apply (erule_tac x = "t1_C.p2_C x'" in allE; clarsimp)
+   apply (drule_tac p = "values_C (heap_WordArray_u32_C st (t1_C.p1_C x')) +\<^sub>p uint (t1_C.p2_C x')" and
                    uv = "UPrim (LU32 x)" in all_heap_rel_ptrD; simp add: type_rel_simp)
   apply clarsimp
   apply (rule_tac x = \<sigma> in exI)
   apply (rule conjI)
    apply (clarsimp simp: \<xi>0_def upd_wordarray_get_0_def)
-   apply (erule_tac x = "p2_C x'" in allE)
+   apply (erule_tac x = "t1_C.p2_C x'" in allE)
    apply (monad_eq simp: wordarray_get_0'_def word_less_nat_alt word_le_nat_alt)
    apply (clarsimp simp: state_rel_def heap_rel_def heap_rel_ptr_meta heap_rel_ptr_w32_meta)
-   apply (drule_tac p = "p1_C x'" and uv = "UAbstract (WAU32 x11 x12)" in all_heap_rel_ptrD; 
+   apply (drule_tac p = "t1_C.p1_C x'" and uv = "UAbstract (WAU32 x11 x12)" in all_heap_rel_ptrD; 
           clarsimp simp: type_rel_simp abs_repr_u_def val_rel_simp is_valid_simp heap_simp)
-   apply (drule_tac p = "values_C (heap_WordArray_u32_C st (p1_C x')) +\<^sub>p uint (p2_C x')" and
+   apply (drule_tac p = "values_C (heap_WordArray_u32_C st (t1_C.p1_C x')) +\<^sub>p uint (t1_C.p2_C x')" and
                    uv = "UPrim (LU32 x)" in all_heap_rel_ptrD;
           clarsimp simp: type_rel_simp val_rel_simp)
   apply (monad_eq simp: wordarray_get_0'_def)
   apply blast
-  done
-
-lemma upd_C_wordarray_get_corres':
-"\<And>i \<gamma> v' \<Gamma>' \<sigma> st.
-    \<lbrakk>i < length \<gamma>; val_rel (\<gamma> ! i) v'; \<Gamma>' ! i = option.Some (prod.fst (prod.snd wordarray_get_0_type))\<rbrakk>
-    \<Longrightarrow> update_sem_init.corres abs_typing_u abs_repr_u (Generated.state_rel abs_repr_u) (App (AFun ''wordarray_get_0'' []) (Var i))
-         (do x <- main_pp_inferred.wordarray_get_0' v';
-             gets (\<lambda>s. x)
-          od)
-         \<xi>0 \<gamma>
-         (assoc_lookup
-           [(''wordarray_get_0'', wordarray_get_0_type), (''wordarray_length_0'', wordarray_length_0_type),
-            (''wordarray_put2_0'', wordarray_put2_0_type), (''wordarray_get_u32'', Generated_TypeProof.wordarray_get_u32_type),
-            (''wordarray_length_u32'', Generated_TypeProof.wordarray_length_u32_type),
-            (''wordarray_put2_u32'', Generated_TypeProof.wordarray_put2_u32_type)]
-           ([], TUnit, TUnit))
-         \<Gamma>' \<sigma> st"
-  apply (insert upd_C_wordarray_get_corres)
-  apply (force simp: \<Xi>_def)
   done
 
 
@@ -1337,5 +1038,156 @@ theorem shallow_C_wordarray_get_strong:
                 upd_proc_env_matches_ptrs_\<xi>0_\<Xi>)
   apply (rule shallow_C_wordarray_get_corres; simp)
   done
+
+thm val_rel_simp
+find_theorems "cogent_function_val_rel"
+
+theorem
+"\<lbrakk>\<And>i \<gamma> v' \<Gamma>' \<sigma>' st.
+    \<lbrakk>i < length \<gamma>; val_rel (\<gamma> ! i) v'; \<Gamma>' ! i = option.Some (prod.fst (prod.snd (\<Xi> ''wordarray_length_0'')))\<rbrakk>
+    \<Longrightarrow> update_sem_init.corres abs_typing_u abs_repr_u (Generated.state_rel abs_repr_u) (App (AFun ''wordarray_length_0'' []) (Var i))
+         (do x <- main_pp_inferred.wordarray_length_0' v';
+             gets (\<lambda>s. x)
+          od)
+         \<xi>0 \<gamma> \<Xi>  \<Gamma>' \<sigma>' st;
+ \<And>v' i \<gamma> \<Gamma> \<sigma> s.
+    \<lbrakk>t5_C.f_C v' = FUN_ENUM_sum; i < length \<gamma>; val_rel (\<gamma> ! i) v';
+     \<Gamma> ! i = option.Some (prod.fst (prod.snd (\<Xi> ''wordarray_fold_no_break_0'')))\<rbrakk>
+    \<Longrightarrow> update_sem_init.corres abs_typing_u abs_repr_u (Generated.state_rel abs_repr_u)
+         (App (AFun ''wordarray_fold_no_break_0'' []) (Var i)) (do x <- main_pp_inferred.wordarray_fold_no_break_0' v';
+gets (\<lambda>s. x)
+                                                                od)
+         \<xi>0 \<gamma> \<Xi>  \<Gamma> \<sigma> s;
+ value_sem.rename_mono_prog abs_typing_v rename \<Xi> \<xi>m \<xi>p;
+ vv\<^sub>m = value_sem.rename_val rename (value_sem.monoval vv\<^sub>p);
+ correspondence_init.val_rel_shallow_C abs_repr_u abs_upd_val' rename vv\<^sub>s uv\<^sub>C vv\<^sub>p uv\<^sub>m \<xi>p \<sigma> \<Xi>; proc_ctx_wellformed \<Xi>;
+ value_sem.proc_env_matches abs_typing_v \<xi>m \<Xi>;
+ value_sem.matches abs_typing_v \<Xi> [vv\<^sub>m] [option.Some (prod.fst (prod.snd Generated_TypeProof.sum_arr_type))]\<rbrakk>
+\<Longrightarrow> correspondence_init.corres_shallow_C abs_repr_u abs_typing_u abs_upd_val' rename (Generated.state_rel abs_repr_u)
+     (Generated_Shallow_Desugar.sum_arr vv\<^sub>s) Generated_TypeProof.sum_arr (main_pp_inferred.sum_arr' uv\<^sub>C) \<xi>0 \<xi>m \<xi>p
+     [uv\<^sub>m] [vv\<^sub>m] \<Xi> [option.Some (prod.fst (prod.snd Generated_TypeProof.sum_arr_type))] \<sigma> s"
+  apply (monad_eq simp: sum_arr'_def  corres_shallow_C_def)
+  apply (frule val_rel_shallow_C_elim(1))
+  
+  oops
+
+lemma
+" \<And>v' i \<gamma> \<Gamma>' \<sigma> s.
+    \<lbrakk>t5_C.f_C v' = FUN_ENUM_sum; i < length \<gamma>; val_rel (\<gamma> ! i) v';
+     \<Gamma>' ! i = option.Some (prod.fst (prod.snd (\<Xi> ''wordarray_fold_no_break_0'')))\<rbrakk>
+    \<Longrightarrow> update_sem_init.corres abs_typing_u abs_repr_u (Generated.state_rel abs_repr_u)
+         (App (AFun ''wordarray_fold_no_break_0'' []) (Var i)) (do x <- main_pp_inferred.wordarray_fold_no_break_0' v';
+gets (\<lambda>s. x)
+                                                                od)
+         \<xi>0 \<gamma> \<Xi>  \<Gamma>' \<sigma> s"
+
+  apply (clarsimp simp: corres_def')
+  apply (frule_tac i = i and 
+                   \<tau> = "prod.fst (prod.snd (\<Xi> ''wordarray_fold_no_break_0''))" in upd.matches_ptrs_proj_single')
+    apply (frule upd.matches_ptrs_length, simp)
+   apply simp
+  apply (clarsimp simp: val_rel_simp)
+  apply (clarsimp simp: cogent_function_val_rel
+                        FUN_ENUM_sum_def
+                        FUN_ENUM_dec_def
+                        FUN_ENUM_inc_def
+                        FUN_ENUM_mul_def
+                        FUN_ENUM_dec_arr_def
+                        FUN_ENUM_inc_arr_def
+                        FUN_ENUM_mul_arr_def
+                        FUN_ENUM_sum_arr_def
+                        FUN_ENUM_wordarray_get_0_def
+                        FUN_ENUM_wordarray_length_0_def
+                        FUN_ENUM_wordarray_put2_0_def
+                        FUN_ENUM_wordarray_fold_no_break_0_def
+                        FUN_ENUM_wordarray_map_no_break_0_def
+                        FUN_ENUM_wordarray_get_u32_def
+                        FUN_ENUM_wordarray_length_u32_def
+                        FUN_ENUM_wordarray_put2_u32_def)
+(*
+  apply (erule upd.u_t_recE)
+  apply (clarsimp simp: \<Xi>_def wordarray_fold_no_break_0_type_def abbreviatedType1_def)
+  apply (erule upd.u_t_r_consE; clarsimp)
+  apply (erule upd.u_t_p_absE; clarsimp simp: abs_typing_u_def)
+  apply (case_tac a; clarsimp)
+  apply (erule upd.u_t_r_consE; clarsimp)
+  apply (erule upd.u_t_primE; subst (asm) lit_type.simps; clarsimp)
+  apply (erule upd.u_t_r_consE; clarsimp)
+  apply (erule upd.u_t_primE; subst (asm) lit_type.simps; clarsimp)
+  apply (erule upd.u_t_r_consE; clarsimp)
+  apply (erule upd.u_t_functionE; clarsimp)
+  apply (erule upd.u_t_r_consE; clarsimp)
+  apply (erule upd.u_t_primE; subst (asm) lit_type.simps; clarsimp)
+  apply (erule upd.u_t_r_consE; clarsimp)
+  apply (erule upd.u_t_r_emptyE)
+  apply (erule upd.u_t_unitE)
+*)
+  apply (clarsimp simp: wordarray_fold_no_break_0'_def)
+  apply wp
+(*
+  apply (rule conjI; clarsimp)
+   apply (monad_eq simp: wordarray_fold_no_break_0'_def)
+
+
+  find_theorems "whileLoop"
+  find_theorems "whileLoopME"
+   prefer 2
+   apply (rule_tac x = \<sigma> in exI)
+   apply (rule conjI)
+    apply (rule u_sem_abs_app)
+      apply (rule u_sem_afun)
+     apply (rule u_sem_var)
+    apply clarsimp
+
+*)
+
+(*
+  apply (rule afun_corres; simp)
+  apply (clarsimp simp: abs_rel_def; rename_tac r w)
+  apply (thin_tac "i < length \<gamma>")
+  apply (thin_tac "val_rel (\<gamma> ! i) v'")
+  apply (thin_tac "\<Gamma>' ! i = option.Some (prod.fst (prod.snd (\<Xi> ''wordarray_fold_no_break_0'')))")
+  apply (clarsimp simp: val_rel_simp \<Xi>_def wordarray_fold_no_break_0_type_def abbreviatedType1_def)
+  apply (erule upd.u_t_recE)
+  apply clarsimp
+  apply (erule upd.u_t_r_consE; clarsimp)+
+  apply (erule upd.u_t_r_emptyE)
+  apply (erule upd.u_t_primE; subst (asm) lit_type.simps; clarsimp)+
+  apply (erule upd.u_t_unitE)
+  apply (erule upd.u_t_p_absE; clarsimp simp: abs_typing_u_def)
+  apply (case_tac a; clarsimp)
+  thm cogent_function_val_rel
+  apply (clarsimp simp: cogent_function_val_rel)
+  apply (erule disjE)+
+   apply clarsimp
+   apply (erule upd.u_t_functionE)
+   apply (clarsimp simp: Generated_TypeProof.dec_def)
+   apply (erule typing_takeE)+
+   apply clarsimp
+   apply (erule typing_varE)+
+   apply (erule typing_letE)+
+   apply clarsimp
+   apply (erule typing_litE)+
+   apply (erule typing_primE)+
+   apply clarsimp
+   apply (erule typing_all_consE)+
+   apply (erule typing_all_emptyE)
+   apply clarsimp
+   apply (erule typing_varE)+
+   apply clarsimp
+   apply (erule typing_structE)
+   apply (erule typing_all_consE)+
+   apply (erule typing_all_emptyE)
+   apply (erule typing_varE)+
+   apply clarsimp
+   apply (subst (asm)  subtyping_simps)+
+  apply clarsimp
+  
+  *)
+  oops
+  thm whileLoop_to_fold
+  find_theorems "fold"
+
+
 end (* of context *)
 end
